Move BFN into new file.

bf.v
@@ -11,316 +11,278 @@ Import ListNotations.
 
 Load parse.
 
-(* BF Program Type *)
-Inductive BF : Set :=
-| bf_end : BF
-| bf_right : BF -> BF (* > *)
-| bf_left : BF -> BF  (* < *)
-| bf_inc : BF -> BF   (* + *)
-| bf_dec : BF -> BF   (* - *)
-| bf_out : BF -> BF   (* . *)
-| bf_in : BF -> BF    (* , *)
-| bf_loop : BF -> BF -> BF.  (* [...] *)
+Module BF.
 
-Section BFPrinting.
+  (* BF Program Type *)
+  Inductive BF : Set :=
+  | bf_end : BF
+  | bf_right : BF -> BF (* > *)
+  | bf_left : BF -> BF  (* < *)
+  | bf_inc : BF -> BF   (* + *)
+  | bf_dec : BF -> BF   (* - *)
+  | bf_out : BF -> BF   (* . *)
+  | bf_in : BF -> BF    (* , *)
+  | bf_loop : BF -> BF -> BF.  (* [...] *)
 
-  Function chars_of_bf (bf: BF): list ascii :=
-    match bf with
-    | bf_end => []
-    | bf_right bf' =>  ">"%char :: (chars_of_bf bf')
-    | bf_left bf' => "<"%char :: (chars_of_bf bf')
-    | bf_inc bf' => "+"%char :: (chars_of_bf bf')
-    | bf_dec bf' => "-"%char :: (chars_of_bf bf')
-    | bf_out bf' => "."%char :: (chars_of_bf bf')
-    | bf_in bf' => ","%char :: (chars_of_bf bf')
-    | bf_loop inner bf' =>
-      "["%char :: (chars_of_bf inner) ++ ["]"%char] ++ (chars_of_bf bf')
-    end.
+  Section BFPrinting.
 
-  Function print_bf (bf: BF): string :=
-    Parse.string_of_chars (chars_of_bf bf).
+    Function chars_of_bf (bf: BF): list ascii :=
+      match bf with
+      | bf_end => []
+      | bf_right bf' =>  ">"%char :: (chars_of_bf bf')
+      | bf_left bf' => "<"%char :: (chars_of_bf bf')
+      | bf_inc bf' => "+"%char :: (chars_of_bf bf')
+      | bf_dec bf' => "-"%char :: (chars_of_bf bf')
+      | bf_out bf' => "."%char :: (chars_of_bf bf')
+      | bf_in bf' => ","%char :: (chars_of_bf bf')
+      | bf_loop inner bf' =>
+        "["%char :: (chars_of_bf inner) ++ ["]"%char] ++ (chars_of_bf bf')
+      end.
 
-  Example print_all_bf_commands:
-    print_bf
-      (bf_loop
-         (bf_right (bf_left (bf_inc (bf_dec (bf_out (bf_in bf_end))))))
-         bf_end)
-    = "[><+-.,]"%string. auto.
+    Function print_bf (bf: BF): string :=
+      Parse.string_of_chars (chars_of_bf bf).
+
+    Example print_all_bf_commands:
+      print_bf
+        (bf_loop
+           (bf_right (bf_left (bf_inc (bf_dec (bf_out (bf_in bf_end))))))
+           bf_end)
+      = "[><+-.,]"%string. auto.
+    Qed.
+
+  End BFPrinting.
+
+  Section BFParsing.
+
+    Local Definition ParseState := @Parse.ParseState BF.
+    Local Definition chars_of_string := Parse.chars_of_string.
+
+    Function parse_bf_state (l: list ascii): ParseState :=
+      match l with
+      | [] => Parse.ok bf_end []
+      | hd :: tl =>
+        match parse_bf_state tl with
+        | Parse.error => Parse.error
+        | Parse.ok cur stack =>
+          match hd with
+          | ">"%char => Parse.ok (bf_right cur) stack
+          | "<"%char => Parse.ok (bf_left cur) stack
+          | "+"%char => Parse.ok (bf_inc cur) stack
+          | "-"%char => Parse.ok (bf_dec cur) stack
+          | "."%char => Parse.ok (bf_out cur) stack
+          | ","%char => Parse.ok (bf_in cur) stack
+          | "]"%char => Parse.ok bf_end (cur :: stack)
+          | "["%char =>
+            match stack with
+            | [] => Parse.error
+            | next :: stack' => Parse.ok (bf_loop cur next) stack'
+            end
+          | _ => Parse.ok cur stack
+          end
+        end
+      end.
+
+    Function parse_bf (str: string): option BF :=
+      match parse_bf_state (chars_of_string str) with
+      | Parse.error => None
+      | Parse.ok _ (_ :: _) => None
+      | Parse.ok bf [] => Some bf
+      end.
+
+    Example parse_all_bf_commands:
+      parse_bf "[><+-.,]" =
+      Some (bf_loop
+              (bf_right (bf_left (bf_inc (bf_dec (bf_out (bf_in bf_end))))))
+              bf_end).
+    auto. Qed.
+
+    Example parse_nesting_bf:
+      parse_bf "[[[][]]][]" =
+      Some (bf_loop
+              (bf_loop
+                 (bf_loop bf_end (bf_loop bf_end bf_end))
+                 bf_end)
+              (bf_loop bf_end bf_end)).
+    auto. Qed.
+
+    Example parse_empty_bf:
+      parse_bf EmptyString = Some bf_end.
+    auto. Qed.
+
+    Example parse_bf_bad_left:
+      parse_bf "[[]" = None.
+    auto. Qed.
+
+    Example parse_bf_bad_right:
+      parse_bf "[]]" = None.
+    auto. Qed.
+
+  End BFParsing.
+
+  Lemma bf_helper (bf1 bf1': BF):
+    parse_bf_state (chars_of_bf bf1) = Parse.ok bf1' [] ->
+    bf1 = bf1'.
+  Proof.
+  Admitted.
+
+  Lemma bf_print_parse_loop (bf1 bf2: BF):
+    forall bf1' bf2',
+      parse_bf_state (chars_of_bf bf1) = Parse.ok bf1' [] ->
+      parse_bf_state (chars_of_bf bf2) = Parse.ok bf2' [] ->
+      parse_bf_state ("["%char :: (chars_of_bf bf1) ++ ["]"%char]
+                         ++ (chars_of_bf bf2))
+      = Parse.ok (bf_loop bf1 bf2) [].
+  Proof.
+  Admitted.
+
+  Lemma bf_print_parse_chars_inv (bf: BF):
+    parse_bf_state (chars_of_bf bf) = Parse.ok bf [].
+  Proof.
+    induction bf; auto;
+      rewrite chars_of_bf_equation, parse_bf_state_equation;
+      try (rewrite IHbf; auto).
+    now apply (bf_print_parse_loop _ _ bf1 bf2).
   Qed.
 
-End BFPrinting.
+  (* Removes the parser from the trusted computing base *)
+  Theorem bf_print_parse_inv (bf: BF): parse_bf (print_bf bf) = Some bf.
+  Proof.
+    unfold parse_bf, print_bf; rewrite Parse.chars_of_string_of_chars_inv.
+    now rewrite bf_print_parse_chars_inv.
+  Qed.
 
-Section BFParsing.
+  (* BF Interpreter *)
+  (* A BFTape is a map from [nat] indices to [Z] values *)
+  Module NatMap := FMapList.Make Nat_as_OT.
+  Definition BFTape := NatMap.t Z.
 
-  Local Definition ParseState := @Parse.ParseState BF.
-  Local Definition chars_of_string := Parse.chars_of_string.
-
-  Function parse_bf_state (l: list ascii): ParseState :=
-    match l with
-    | [] => Parse.ok bf_end []
-    | hd :: tl =>
-      match parse_bf_state tl with
-      | Parse.error => Parse.error
-      | Parse.ok cur stack =>
-        match hd with
-        | ">"%char => Parse.ok (bf_right cur) stack
-        | "<"%char => Parse.ok (bf_left cur) stack
-        | "+"%char => Parse.ok (bf_inc cur) stack
-        | "-"%char => Parse.ok (bf_dec cur) stack
-        | "."%char => Parse.ok (bf_out cur) stack
-        | ","%char => Parse.ok (bf_in cur) stack
-        | "]"%char => Parse.ok bf_end (cur :: stack)
-        | "["%char =>
-          match stack with
-          | [] => Parse.error
-          | next :: stack' => Parse.ok (bf_loop cur next) stack'
-          end
-        | _ => Parse.ok cur stack
-        end
-      end
+  Definition tape_get (tape: BFTape) (ptr: nat): Z :=
+    match (NatMap.find ptr tape) with
+    | Some x => x
+    | None => 0
     end.
 
-  Function parse_bf (str: string): option BF :=
-    match parse_bf_state (chars_of_string str) with
-    | Parse.error => None
-    | Parse.ok _ (_ :: _) => None
-    | Parse.ok bf [] => Some bf
-    end.
+  Definition tape_set (tape: BFTape) (ptr: nat) (x: Z): BFTape :=
+    NatMap.add ptr x tape.
 
-  Example parse_all_bf_commands:
-    parse_bf "[><+-.,]" =
-    Some (bf_loop
-            (bf_right (bf_left (bf_inc (bf_dec (bf_out (bf_in bf_end))))))
-            bf_end).
-  auto. Qed.
+  Definition tape_inc (tape: BFTape) (ptr: nat): BFTape :=
+    tape_set tape ptr (Z.succ (tape_get tape ptr)).
 
-  Example parse_nesting_bf:
-    parse_bf "[[[][]]][]" =
-    Some (bf_loop
-            (bf_loop
-               (bf_loop bf_end (bf_loop bf_end bf_end))
-               bf_end)
-            (bf_loop bf_end bf_end)).
-  auto. Qed.
+  Definition tape_dec (tape: BFTape) (ptr: nat): BFTape :=
+    tape_set tape ptr (Z.pred (tape_get tape ptr)).
 
-  Example parse_empty_bf:
-    parse_bf EmptyString = Some bf_end.
-  auto. Qed.
+  (* `bf' is the current state of the program, while `resets' is the
+     stack of programs to reset to at the end of a loop *)
+  (* TODO: Generalize to all tape languages *)
+  Inductive BFState : Type :=
+    bf_state (bf: BF)
+             (resets: list BF)
+             (ptr: nat)
+             (tape: BFTape)
+             (input: list Z)
+             (output: list Z).
 
-  Example parse_bf_bad_left:
-    parse_bf "[[]" = None.
-  auto. Qed.
+  Function bf_state_init (bf: BF) (input: list Z): BFState :=
+    bf_state bf [] 0 (NatMap.empty Z) input [].
 
-  Example parse_bf_bad_right:
-    parse_bf "[]]" = None.
-  auto. Qed.
+  Function bf_state_output (state: BFState): list Z :=
+    match state with bf_state _ _ _ _ _ output => output end.
 
-End BFParsing.
-
-Lemma bf_helper (bf1 bf1': BF):
-  parse_bf_state (chars_of_bf bf1) = Parse.ok bf1' [] ->
-  bf1 = bf1'.
-Proof.
-Admitted.
-
-Lemma bf_print_parse_loop (bf1 bf2: BF):
-  forall bf1' bf2',
-    parse_bf_state (chars_of_bf bf1) = Parse.ok bf1' [] ->
-    parse_bf_state (chars_of_bf bf2) = Parse.ok bf2' [] ->
-    parse_bf_state ("["%char :: (chars_of_bf bf1) ++ ["]"%char]
-                                  ++ (chars_of_bf bf2))
-    = Parse.ok (bf_loop bf1 bf2) [].
-Proof.
-Admitted.
-
-Lemma bf_print_parse_chars_inv (bf: BF):
-  parse_bf_state (chars_of_bf bf) = Parse.ok bf [].
-Proof.
-  induction bf; auto;
-    rewrite chars_of_bf_equation, parse_bf_state_equation;
-    try (rewrite IHbf; auto).
-  now apply (bf_print_parse_loop _ _ bf1 bf2).
-Qed.
-
-(* Removes the parser from the trusted computing base *)
-Theorem bf_print_parse_inv (bf: BF): parse_bf (print_bf bf) = Some bf.
-Proof.
-  unfold parse_bf, print_bf; rewrite Parse.chars_of_string_of_chars_inv.
-  now rewrite bf_print_parse_chars_inv.
-Qed.
-
-(* BF Interpreter *)
-(* A BFTape is a map from [nat] indices to [Z] values *)
-Module NatMap := FMapList.Make Nat_as_OT.
-Definition BFTape := NatMap.t Z.
-
-Definition tape_get (tape: BFTape) (ptr: nat): Z :=
-  match (NatMap.find ptr tape) with
-  | Some x => x
-  | None => 0
-  end.
-
-Definition tape_set (tape: BFTape) (ptr: nat) (x: Z): BFTape :=
-  NatMap.add ptr x tape.
-
-Definition tape_inc (tape: BFTape) (ptr: nat): BFTape :=
-  tape_set tape ptr (Z.succ (tape_get tape ptr)).
-
-Definition tape_dec (tape: BFTape) (ptr: nat): BFTape :=
-  tape_set tape ptr (Z.pred (tape_get tape ptr)).
-
-(* `bf' is the current state of the program, while `resets' is the
-stack of programs to reset to at the end of a loop *)
-(* TODO: Generalize to all tape languages *)
-Inductive BFState : Type :=
-  bf_state (bf: BF)
-           (resets: list BF)
-           (ptr: nat)
-           (tape: BFTape)
-           (input: list Z)
-           (output: list Z).
-
-Function bf_state_init (bf: BF) (input: list Z): BFState :=
-  bf_state bf [] 0 (NatMap.empty Z) input [].
-
-Function bf_state_output (state: BFState): list Z :=
-  match state with bf_state _ _ _ _ _ output => output end.
-
-Function bf_step (state: BFState): option BFState :=
-  match state with
-  | bf_state bf resets ptr tape input output =>
-    match bf with
-     | bf_end =>
-       match resets with
+  Function bf_step (state: BFState): option BFState :=
+    match state with
+    | bf_state bf resets ptr tape input output =>
+      match bf with
+      | bf_end =>
+        match resets with
         | [] => None
         | bf' :: resets' =>
           Some (bf_state bf' resets' ptr tape input output)
         end
-     | bf_right bf' =>
-       Some (bf_state bf' resets (S ptr) tape input output)
-     | bf_left bf' =>
-       Some (bf_state bf' resets (pred ptr) tape input output)
-     | bf_inc bf' =>
-       Some (bf_state bf' resets ptr (tape_inc tape ptr) input output)
-     | bf_dec bf' =>
-       Some (bf_state bf' resets ptr (tape_dec tape ptr) input output)
-     | bf_out bf' =>
-       Some (bf_state bf' resets ptr tape input (output ++ [tape_get tape ptr]))
-     | bf_in bf' =>
-       match input with
+      | bf_right bf' =>
+        Some (bf_state bf' resets (S ptr) tape input output)
+      | bf_left bf' =>
+        Some (bf_state bf' resets (pred ptr) tape input output)
+      | bf_inc bf' =>
+        Some (bf_state bf' resets ptr (tape_inc tape ptr) input output)
+      | bf_dec bf' =>
+        Some (bf_state bf' resets ptr (tape_dec tape ptr) input output)
+      | bf_out bf' =>
+        Some (bf_state bf' resets ptr tape input (output ++ [tape_get tape ptr]))
+      | bf_in bf' =>
+        match input with
         | [] =>
           Some (bf_state bf' resets ptr (tape_set tape ptr 0) input output)
         | x :: input' =>
           Some (bf_state bf' resets ptr (tape_set tape ptr x) input' output)
         end
-     | bf_loop inner_bf bf' =>
-       if Z.eqb (tape_get tape ptr) Z.zero then
-         Some (bf_state bf' resets ptr tape input output)
-       else
+      | bf_loop inner_bf bf' =>
+        if Z.eqb (tape_get tape ptr) Z.zero then
+          Some (bf_state bf' resets ptr tape input output)
+        else
           Some (bf_state inner_bf (bf :: resets) ptr tape input output)
-     end
-  end.
+      end
+    end.
 
-(* TODO: Use N as fuel with {measure N.to_nat fuel} *)
-Function bf_run (state: BFState) (fuel: nat): option (list Z) :=
-  match fuel with
-  | 0 => None
-  | S f =>
-    match bf_step state with
-    | None => Some (bf_state_output state)
-    | Some state' => bf_run state' f
-    end
-  end.
+  (* TODO: Use N as fuel with {measure N.to_nat fuel} *)
+  Function bf_run (state: BFState) (fuel: nat): option (list Z) :=
+    match fuel with
+    | 0 => None
+    | S f =>
+      match bf_step state with
+      | None => Some (bf_state_output state)
+      | Some state' => bf_run state' f
+      end
+    end.
 
-Function z_of_ascii (a: ascii): Z :=
-  Z.of_nat (nat_of_ascii a).
+  Function z_of_ascii (a: ascii): Z :=
+    Z.of_nat (nat_of_ascii a).
 
-Function ascii_of_z (z: Z): option ascii :=
-  match z with
-  | Zpos p => Some (ascii_of_pos p)
-  | _ => None
-  end.
+  Function ascii_of_z (z: Z): option ascii :=
+    match z with
+    | Zpos p => Some (ascii_of_pos p)
+    | _ => None
+    end.
 
-Function opt_list_len {A: Type} (l: option (list A)): nat :=
-  match l with
-  | Some l => List.length l
-  | None => 0
-  end.
+  Function opt_list_len {A: Type} (l: option (list A)): nat :=
+    match l with
+    | Some l => List.length l
+    | None => 0
+    end.
 
-Function string_of_zs (out: list Z): string :=
-  match out with
-  | [] => EmptyString
-  | z :: zs' =>
-    match ascii_of_z z with
+  Function string_of_zs (out: list Z): string :=
+    match out with
+    | [] => EmptyString
+    | z :: zs' =>
+      match ascii_of_z z with
+      | None => EmptyString
+      | Some a => String a (string_of_zs zs')
+      end
+    end.
+
+  Function zs_of_string (str: string): list Z :=
+    match str with
+    | EmptyString => []
+    | String a str' => z_of_ascii a :: (zs_of_string str')
+    end.
+
+  (* The important interpreter as far as the spec is concerned *)
+  Function interpret_bf (prog: string) (zs: list Z) (f: nat): option (list Z) :=
+    match parse_bf prog with
+    | None => None
+    | Some bf => bf_run (bf_state_init bf zs) f
+    end.
+
+  Function interpret_bf_readable (prog: string) (input: string) (f:nat):
+    string :=
+    match interpret_bf prog (zs_of_string input) f with
     | None => EmptyString
-    | Some a => String a (string_of_zs zs')
-    end
-  end.
+    | Some zs => string_of_zs zs
+    end.
 
-Function zs_of_string (str: string): list Z :=
-  match str with
-  | EmptyString => []
-  | String a str' => z_of_ascii a :: (zs_of_string str')
-  end.
-
-(* The important interpreter as far as the spec is concerned *)
-Function interpret_bf (prog: string) (zs: list Z) (f: nat): option (list Z) :=
-  match parse_bf prog with
-  | None => None
-  | Some bf => bf_run (bf_state_init bf zs) f
-  end.
-
-Function interpret_bf_readable (prog: string) (input: string) (f:nat): string :=
-  match interpret_bf prog (zs_of_string input) f with
-  | None => EmptyString
-  | Some zs => string_of_zs zs
-  end.
-
-Example hello_world_bf:
-  interpret_bf_readable "++++++++++[>+++++++>++++++++++>+++>+<<<<-]>++.>+.
+  Example hello_world_bf:
+    interpret_bf_readable "++++++++++[>+++++++>++++++++++>+++>+<<<<-]>++.>+.
                         +++++++..+++.>++.<<+++++++++++++++.>.+++.------.
                         --------.>+. newline in next cell" "" 401 =
-  "Hello World!"%string. Proof. auto. Qed.
+    "Hello World!"%string. Proof. auto. Qed.
 
-
-
-Section BFN.
-
-(* Layer 1 above BF: BFN Program Type. Repeat each command N times *)
-Inductive BFN : Set :=
-| bfn_end : BFN
-| bfn_right : nat -> BFN -> BFN (* > *)
-| bfn_left : nat -> BFN -> BFN  (* < *)
-| bfn_inc : nat -> BFN -> BFN   (* + *)
-| bfn_dec : nat -> BFN -> BFN   (* - *)
-| bfn_out : nat -> BFN -> BFN   (* . *)
-| bfn_in : nat -> BFN -> BFN    (* , *)
-| bfn_loop : BFN -> BFN -> BFN.  (* [...] *)
-
-
-Fixpoint repeat (fn : BF -> BF) (n : nat) (bf: BF) : BF :=
-  match n with
-  | 0 => bf_end  (* should probably not be used *)
-  | 1 => fn bf
-  | S m => fn (repeat fn m bf)
-  end.
-
-Fixpoint bfn_to_bf (bfn: BFN): BF :=
-  match bfn with
-  | bfn_end => bf_end
-  | bfn_right n bfn' => repeat bf_right n (bfn_to_bf bfn')
-  | bfn_left n bfn' => repeat bf_left n (bfn_to_bf bfn')
-  | bfn_inc n bfn' => repeat bf_inc n (bfn_to_bf bfn')
-  | bfn_dec n bfn' => repeat bf_dec n (bfn_to_bf bfn')
-  | bfn_out n bfn' => repeat bf_out n (bfn_to_bf bfn')
-  | bfn_in n bfn' => repeat bf_in n (bfn_to_bf bfn')
-  | bfn_loop bfn1 bfn2 => bf_loop (bfn_to_bf bfn1) (bfn_to_bf bfn2)
-  end.
-
-  Example parse_left_bfn:
-    parse_bf "<<<<+++++++" =
-    Some (bfn_to_bf (bfn_left 4 (bfn_inc 7 bfn_end))).
-  auto. Qed.
-
-End BFN.
-
+End BF.
